Define vectors and prove validity

theories/CastRemoval.v
@@ -32,6 +32,10 @@ Equations castrm : term → term := {
   ε| tzero | := tzero ;
   ε| tsucc n | := tsucc ε|n| ;
   ε| tnat_elim m n P z s | := tnat_elim m ε|n| ε|P| ε|z| ε|s| ;
+  ε| tvec A n | := tvec ε|A| ε|n| ;
+  ε| tvnil A | := tvnil ε|A| ;
+  ε| tvcons a n v | := tvcons ε|a| ε|n| ε|v| ;
+  ε| tvec_elim m v P z s | := tvec_elim m ε|v| ε|P| ε|z| ε|s| ;
   ε| bot | := bot ;
   ε| bot_elim m A p | := bot_elim m ε|A| ε|p|
 }
