theories/autosubst/GAST.v
@@ -28,6 +28,10 @@ Inductive term : Type :=
   | tzero : term
   | tsucc : term -> term
   | tnat_elim : mode -> term -> term -> term -> term -> term
+  | tvec : term -> term -> term
+  | tvnil : term -> term
+  | tvcons : term -> term -> term -> term
+  | tvec_elim : mode -> term -> term -> term -> term -> term
   | bot : term
   | bot_elim : mode -> term -> term -> term.
 
@@ -223,6 +227,45 @@ exact (eq_trans
          (ap (fun x => tnat_elim t0 t1 t2 t3 x) H4)).
 Qed.
 
+Lemma congr_tvec {s0 : term} {s1 : term} {t0 : term} {t1 : term}
+  (H0 : s0 = t0) (H1 : s1 = t1) : tvec s0 s1 = tvec t0 t1.
+Proof.
+exact (eq_trans (eq_trans eq_refl (ap (fun x => tvec x s1) H0))
+         (ap (fun x => tvec t0 x) H1)).
+Qed.
+
+Lemma congr_tvnil {s0 : term} {t0 : term} (H0 : s0 = t0) :
+  tvnil s0 = tvnil t0.
+Proof.
+exact (eq_trans eq_refl (ap (fun x => tvnil x) H0)).
+Qed.
+
+Lemma congr_tvcons {s0 : term} {s1 : term} {s2 : term} {t0 : term}
+  {t1 : term} {t2 : term} (H0 : s0 = t0) (H1 : s1 = t1) (H2 : s2 = t2) :
+  tvcons s0 s1 s2 = tvcons t0 t1 t2.
+Proof.
+exact (eq_trans
+         (eq_trans (eq_trans eq_refl (ap (fun x => tvcons x s1 s2) H0))
+            (ap (fun x => tvcons t0 x s2) H1))
+         (ap (fun x => tvcons t0 t1 x) H2)).
+Qed.
+
+Lemma congr_tvec_elim {s0 : mode} {s1 : term} {s2 : term} {s3 : term}
+  {s4 : term} {t0 : mode} {t1 : term} {t2 : term} {t3 : term} {t4 : term}
+  (H0 : s0 = t0) (H1 : s1 = t1) (H2 : s2 = t2) (H3 : s3 = t3) (H4 : s4 = t4)
+  : tvec_elim s0 s1 s2 s3 s4 = tvec_elim t0 t1 t2 t3 t4.
+Proof.
+exact (eq_trans
+         (eq_trans
+            (eq_trans
+               (eq_trans
+                  (eq_trans eq_refl (ap (fun x => tvec_elim x s1 s2 s3 s4) H0))
+                  (ap (fun x => tvec_elim t0 x s2 s3 s4) H1))
+               (ap (fun x => tvec_elim t0 t1 x s3 s4) H2))
+            (ap (fun x => tvec_elim t0 t1 t2 x s4) H3))
+         (ap (fun x => tvec_elim t0 t1 t2 t3 x) H4)).
+Qed.
+
 Lemma congr_bot : bot = bot.
 Proof.
 exact (eq_refl).
@@ -284,6 +327,14 @@ Fixpoint ren_term (xi_term : nat -> nat) (s : term) {struct s} : term :=
   | tnat_elim s0 s1 s2 s3 s4 =>
       tnat_elim s0 (ren_term xi_term s1) (ren_term xi_term s2)
         (ren_term xi_term s3) (ren_term xi_term s4)
+  | tvec s0 s1 => tvec (ren_term xi_term s0) (ren_term xi_term s1)
+  | tvnil s0 => tvnil (ren_term xi_term s0)
+  | tvcons s0 s1 s2 =>
+      tvcons (ren_term xi_term s0) (ren_term xi_term s1)
+        (ren_term xi_term s2)
+  | tvec_elim s0 s1 s2 s3 s4 =>
+      tvec_elim s0 (ren_term xi_term s1) (ren_term xi_term s2)
+        (ren_term xi_term s3) (ren_term xi_term s4)
   | bot => bot
   | bot_elim s0 s1 s2 =>
       bot_elim s0 (ren_term xi_term s1) (ren_term xi_term s2)
@@ -294,7 +345,7 @@ Proof.
 exact (scons (var var_zero) (funcomp (ren_term shift) sigma)).
 Defined.
 
-Fixpoint subst_term (sigma_term : nat -> term) (s : term) {struct s} : 
+Fixpoint subst_term (sigma_term : nat -> term) (s : term) {struct s} :
 term :=
   match s with
   | var s0 => sigma_term s0
@@ -340,6 +391,14 @@ term :=
   | tsucc s0 => tsucc (subst_term sigma_term s0)
   | tnat_elim s0 s1 s2 s3 s4 =>
       tnat_elim s0 (subst_term sigma_term s1) (subst_term sigma_term s2)
+        (subst_term sigma_term s3) (subst_term sigma_term s4)
+  | tvec s0 s1 => tvec (subst_term sigma_term s0) (subst_term sigma_term s1)
+  | tvnil s0 => tvnil (subst_term sigma_term s0)
+  | tvcons s0 s1 s2 =>
+      tvcons (subst_term sigma_term s0) (subst_term sigma_term s1)
+        (subst_term sigma_term s2)
+  | tvec_elim s0 s1 s2 s3 s4 =>
+      tvec_elim s0 (subst_term sigma_term s1) (subst_term sigma_term s2)
         (subst_term sigma_term s3) (subst_term sigma_term s4)
   | bot => bot
   | bot_elim s0 s1 s2 =>
@@ -417,6 +476,19 @@ subst_term sigma_term s = s :=
   | tsucc s0 => congr_tsucc (idSubst_term sigma_term Eq_term s0)
   | tnat_elim s0 s1 s2 s3 s4 =>
       congr_tnat_elim (eq_refl s0) (idSubst_term sigma_term Eq_term s1)
+        (idSubst_term sigma_term Eq_term s2)
+        (idSubst_term sigma_term Eq_term s3)
+        (idSubst_term sigma_term Eq_term s4)
+  | tvec s0 s1 =>
+      congr_tvec (idSubst_term sigma_term Eq_term s0)
+        (idSubst_term sigma_term Eq_term s1)
+  | tvnil s0 => congr_tvnil (idSubst_term sigma_term Eq_term s0)
+  | tvcons s0 s1 s2 =>
+      congr_tvcons (idSubst_term sigma_term Eq_term s0)
+        (idSubst_term sigma_term Eq_term s1)
+        (idSubst_term sigma_term Eq_term s2)
+  | tvec_elim s0 s1 s2 s3 s4 =>
+      congr_tvec_elim (eq_refl s0) (idSubst_term sigma_term Eq_term s1)
         (idSubst_term sigma_term Eq_term s2)
         (idSubst_term sigma_term Eq_term s3)
         (idSubst_term sigma_term Eq_term s4)
@@ -503,6 +575,19 @@ ren_term xi_term s = ren_term zeta_term s :=
         (extRen_term xi_term zeta_term Eq_term s2)
         (extRen_term xi_term zeta_term Eq_term s3)
         (extRen_term xi_term zeta_term Eq_term s4)
+  | tvec s0 s1 =>
+      congr_tvec (extRen_term xi_term zeta_term Eq_term s0)
+        (extRen_term xi_term zeta_term Eq_term s1)
+  | tvnil s0 => congr_tvnil (extRen_term xi_term zeta_term Eq_term s0)
+  | tvcons s0 s1 s2 =>
+      congr_tvcons (extRen_term xi_term zeta_term Eq_term s0)
+        (extRen_term xi_term zeta_term Eq_term s1)
+        (extRen_term xi_term zeta_term Eq_term s2)
+  | tvec_elim s0 s1 s2 s3 s4 =>
+      congr_tvec_elim (eq_refl s0) (extRen_term xi_term zeta_term Eq_term s1)
+        (extRen_term xi_term zeta_term Eq_term s2)
+        (extRen_term xi_term zeta_term Eq_term s3)
+        (extRen_term xi_term zeta_term Eq_term s4)
   | bot => congr_bot
   | bot_elim s0 s1 s2 =>
       congr_bot_elim (eq_refl s0) (extRen_term xi_term zeta_term Eq_term s1)
@@ -584,6 +669,19 @@ subst_term sigma_term s = subst_term tau_term s :=
   | tsucc s0 => congr_tsucc (ext_term sigma_term tau_term Eq_term s0)
   | tnat_elim s0 s1 s2 s3 s4 =>
       congr_tnat_elim (eq_refl s0) (ext_term sigma_term tau_term Eq_term s1)
+        (ext_term sigma_term tau_term Eq_term s2)
+        (ext_term sigma_term tau_term Eq_term s3)
+        (ext_term sigma_term tau_term Eq_term s4)
+  | tvec s0 s1 =>
+      congr_tvec (ext_term sigma_term tau_term Eq_term s0)
+        (ext_term sigma_term tau_term Eq_term s1)
+  | tvnil s0 => congr_tvnil (ext_term sigma_term tau_term Eq_term s0)
+  | tvcons s0 s1 s2 =>
+      congr_tvcons (ext_term sigma_term tau_term Eq_term s0)
+        (ext_term sigma_term tau_term Eq_term s1)
+        (ext_term sigma_term tau_term Eq_term s2)
+  | tvec_elim s0 s1 s2 s3 s4 =>
+      congr_tvec_elim (eq_refl s0) (ext_term sigma_term tau_term Eq_term s1)
         (ext_term sigma_term tau_term Eq_term s2)
         (ext_term sigma_term tau_term Eq_term s3)
         (ext_term sigma_term tau_term Eq_term s4)
@@ -675,6 +773,21 @@ Fixpoint compRenRen_term (xi_term : nat -> nat) (zeta_term : nat -> nat)
       congr_tsucc (compRenRen_term xi_term zeta_term rho_term Eq_term s0)
   | tnat_elim s0 s1 s2 s3 s4 =>
       congr_tnat_elim (eq_refl s0)
+        (compRenRen_term xi_term zeta_term rho_term Eq_term s1)
+        (compRenRen_term xi_term zeta_term rho_term Eq_term s2)
+        (compRenRen_term xi_term zeta_term rho_term Eq_term s3)
+        (compRenRen_term xi_term zeta_term rho_term Eq_term s4)
+  | tvec s0 s1 =>
+      congr_tvec (compRenRen_term xi_term zeta_term rho_term Eq_term s0)
+        (compRenRen_term xi_term zeta_term rho_term Eq_term s1)
+  | tvnil s0 =>
+      congr_tvnil (compRenRen_term xi_term zeta_term rho_term Eq_term s0)
+  | tvcons s0 s1 s2 =>
+      congr_tvcons (compRenRen_term xi_term zeta_term rho_term Eq_term s0)
+        (compRenRen_term xi_term zeta_term rho_term Eq_term s1)
+        (compRenRen_term xi_term zeta_term rho_term Eq_term s2)
+  | tvec_elim s0 s1 s2 s3 s4 =>
+      congr_tvec_elim (eq_refl s0)
         (compRenRen_term xi_term zeta_term rho_term Eq_term s1)
         (compRenRen_term xi_term zeta_term rho_term Eq_term s2)
         (compRenRen_term xi_term zeta_term rho_term Eq_term s3)
@@ -773,6 +886,21 @@ subst_term tau_term (ren_term xi_term s) = subst_term theta_term s :=
       congr_tsucc (compRenSubst_term xi_term tau_term theta_term Eq_term s0)
   | tnat_elim s0 s1 s2 s3 s4 =>
       congr_tnat_elim (eq_refl s0)
+        (compRenSubst_term xi_term tau_term theta_term Eq_term s1)
+        (compRenSubst_term xi_term tau_term theta_term Eq_term s2)
+        (compRenSubst_term xi_term tau_term theta_term Eq_term s3)
+        (compRenSubst_term xi_term tau_term theta_term Eq_term s4)
+  | tvec s0 s1 =>
+      congr_tvec (compRenSubst_term xi_term tau_term theta_term Eq_term s0)
+        (compRenSubst_term xi_term tau_term theta_term Eq_term s1)
+  | tvnil s0 =>
+      congr_tvnil (compRenSubst_term xi_term tau_term theta_term Eq_term s0)
+  | tvcons s0 s1 s2 =>
+      congr_tvcons (compRenSubst_term xi_term tau_term theta_term Eq_term s0)
+        (compRenSubst_term xi_term tau_term theta_term Eq_term s1)
+        (compRenSubst_term xi_term tau_term theta_term Eq_term s2)
+  | tvec_elim s0 s1 s2 s3 s4 =>
+      congr_tvec_elim (eq_refl s0)
         (compRenSubst_term xi_term tau_term theta_term Eq_term s1)
         (compRenSubst_term xi_term tau_term theta_term Eq_term s2)
         (compRenSubst_term xi_term tau_term theta_term Eq_term s3)
@@ -895,6 +1023,24 @@ ren_term zeta_term (subst_term sigma_term s) = subst_term theta_term s :=
         (compSubstRen_term sigma_term zeta_term theta_term Eq_term s2)
         (compSubstRen_term sigma_term zeta_term theta_term Eq_term s3)
         (compSubstRen_term sigma_term zeta_term theta_term Eq_term s4)
+  | tvec s0 s1 =>
+      congr_tvec
+        (compSubstRen_term sigma_term zeta_term theta_term Eq_term s0)
+        (compSubstRen_term sigma_term zeta_term theta_term Eq_term s1)
+  | tvnil s0 =>
+      congr_tvnil
+        (compSubstRen_term sigma_term zeta_term theta_term Eq_term s0)
+  | tvcons s0 s1 s2 =>
+      congr_tvcons
+        (compSubstRen_term sigma_term zeta_term theta_term Eq_term s0)
+        (compSubstRen_term sigma_term zeta_term theta_term Eq_term s1)
+        (compSubstRen_term sigma_term zeta_term theta_term Eq_term s2)
+  | tvec_elim s0 s1 s2 s3 s4 =>
+      congr_tvec_elim (eq_refl s0)
+        (compSubstRen_term sigma_term zeta_term theta_term Eq_term s1)
+        (compSubstRen_term sigma_term zeta_term theta_term Eq_term s2)
+        (compSubstRen_term sigma_term zeta_term theta_term Eq_term s3)
+        (compSubstRen_term sigma_term zeta_term theta_term Eq_term s4)
   | bot => congr_bot
   | bot_elim s0 s1 s2 =>
       congr_bot_elim (eq_refl s0)
@@ -1011,6 +1157,24 @@ subst_term tau_term (subst_term sigma_term s) = subst_term theta_term s :=
         (compSubstSubst_term sigma_term tau_term theta_term Eq_term s0)
   | tnat_elim s0 s1 s2 s3 s4 =>
       congr_tnat_elim (eq_refl s0)
+        (compSubstSubst_term sigma_term tau_term theta_term Eq_term s1)
+        (compSubstSubst_term sigma_term tau_term theta_term Eq_term s2)
+        (compSubstSubst_term sigma_term tau_term theta_term Eq_term s3)
+        (compSubstSubst_term sigma_term tau_term theta_term Eq_term s4)
+  | tvec s0 s1 =>
+      congr_tvec
+        (compSubstSubst_term sigma_term tau_term theta_term Eq_term s0)
+        (compSubstSubst_term sigma_term tau_term theta_term Eq_term s1)
+  | tvnil s0 =>
+      congr_tvnil
+        (compSubstSubst_term sigma_term tau_term theta_term Eq_term s0)
+  | tvcons s0 s1 s2 =>
+      congr_tvcons
+        (compSubstSubst_term sigma_term tau_term theta_term Eq_term s0)
+        (compSubstSubst_term sigma_term tau_term theta_term Eq_term s1)
+        (compSubstSubst_term sigma_term tau_term theta_term Eq_term s2)
+  | tvec_elim s0 s1 s2 s3 s4 =>
+      congr_tvec_elim (eq_refl s0)
         (compSubstSubst_term sigma_term tau_term theta_term Eq_term s1)
         (compSubstSubst_term sigma_term tau_term theta_term Eq_term s2)
         (compSubstSubst_term sigma_term tau_term theta_term Eq_term s3)
@@ -1168,6 +1332,20 @@ Fixpoint rinst_inst_term (xi_term : nat -> nat) (sigma_term : nat -> term)
         (rinst_inst_term xi_term sigma_term Eq_term s2)
         (rinst_inst_term xi_term sigma_term Eq_term s3)
         (rinst_inst_term xi_term sigma_term Eq_term s4)
+  | tvec s0 s1 =>
+      congr_tvec (rinst_inst_term xi_term sigma_term Eq_term s0)
+        (rinst_inst_term xi_term sigma_term Eq_term s1)
+  | tvnil s0 => congr_tvnil (rinst_inst_term xi_term sigma_term Eq_term s0)
+  | tvcons s0 s1 s2 =>
+      congr_tvcons (rinst_inst_term xi_term sigma_term Eq_term s0)
+        (rinst_inst_term xi_term sigma_term Eq_term s1)
+        (rinst_inst_term xi_term sigma_term Eq_term s2)
+  | tvec_elim s0 s1 s2 s3 s4 =>
+      congr_tvec_elim (eq_refl s0)
+        (rinst_inst_term xi_term sigma_term Eq_term s1)
+        (rinst_inst_term xi_term sigma_term Eq_term s2)
+        (rinst_inst_term xi_term sigma_term Eq_term s3)
+        (rinst_inst_term xi_term sigma_term Eq_term s4)
   | bot => congr_bot
   | bot_elim s0 s1 s2 =>
       congr_bot_elim (eq_refl s0)
@@ -1315,7 +1493,7 @@ Tactic Notation "auto_unfold" "in" "*" := repeat
                                            unfold VarInstance_term, Var, ids,
                                             Ren_term, Ren1, ren1,
                                             Up_term_term, Up_term, up_term,
-                                            Subst_term, Subst1, subst1 
+                                            Subst_term, Subst1, subst1
                                             in *.
 
 Ltac asimpl' := repeat (first
@@ -1426,6 +1604,17 @@ Fixpoint allfv_term (p_term : nat -> Prop) (s : term) {struct s} : Prop :=
         (and (allfv_term p_term s1)
            (and (allfv_term p_term s2)
               (and (allfv_term p_term s3) (and (allfv_term p_term s4) True))))
+  | tvec s0 s1 =>
+      and (allfv_term p_term s0) (and (allfv_term p_term s1) True)
+  | tvnil s0 => and (allfv_term p_term s0) True
+  | tvcons s0 s1 s2 =>
+      and (allfv_term p_term s0)
+        (and (allfv_term p_term s1) (and (allfv_term p_term s2) True))
+  | tvec_elim s0 s1 s2 s3 s4 =>
+      and True
+        (and (allfv_term p_term s1)
+           (and (allfv_term p_term s2)
+              (and (allfv_term p_term s3) (and (allfv_term p_term s4) True))))
   | bot => True
   | bot_elim s0 s1 s2 =>
       and True (and (allfv_term p_term s1) (and (allfv_term p_term s2) True))
@@ -1510,6 +1699,20 @@ Fixpoint allfvTriv_term (p_term : nat -> Prop) (H_term : forall x, p_term x)
   | tzero => I
   | tsucc s0 => conj (allfvTriv_term p_term H_term s0) I
   | tnat_elim s0 s1 s2 s3 s4 =>
+      conj I
+        (conj (allfvTriv_term p_term H_term s1)
+           (conj (allfvTriv_term p_term H_term s2)
+              (conj (allfvTriv_term p_term H_term s3)
+                 (conj (allfvTriv_term p_term H_term s4) I))))
+  | tvec s0 s1 =>
+      conj (allfvTriv_term p_term H_term s0)
+        (conj (allfvTriv_term p_term H_term s1) I)
+  | tvnil s0 => conj (allfvTriv_term p_term H_term s0) I
+  | tvcons s0 s1 s2 =>
+      conj (allfvTriv_term p_term H_term s0)
+        (conj (allfvTriv_term p_term H_term s1)
+           (conj (allfvTriv_term p_term H_term s2) I))
+  | tvec_elim s0 s1 s2 s3 s4 =>
       conj I
         (conj (allfvTriv_term p_term H_term s1)
            (conj (allfvTriv_term p_term H_term s2)
@@ -1911,6 +2114,102 @@ allfv_term p_term s -> allfv_term q_term s :=
            | conj HP _ => HP
            end) I
   | tnat_elim s0 s1 s2 s3 s4 =>
+      fun HP =>
+      conj I
+        (conj
+           (allfvImpl_term p_term q_term H_term s1
+              match HP with
+              | conj _ HP => match HP with
+                             | conj HP _ => HP
+                             end
+              end)
+           (conj
+              (allfvImpl_term p_term q_term H_term s2
+                 match HP with
+                 | conj _ HP =>
+                     match HP with
+                     | conj _ HP => match HP with
+                                    | conj HP _ => HP
+                                    end
+                     end
+                 end)
+              (conj
+                 (allfvImpl_term p_term q_term H_term s3
+                    match HP with
+                    | conj _ HP =>
+                        match HP with
+                        | conj _ HP =>
+                            match HP with
+                            | conj _ HP =>
+                                match HP with
+                                | conj HP _ => HP
+                                end
+                            end
+                        end
+                    end)
+                 (conj
+                    (allfvImpl_term p_term q_term H_term s4
+                       match HP with
+                       | conj _ HP =>
+                           match HP with
+                           | conj _ HP =>
+                               match HP with
+                               | conj _ HP =>
+                                   match HP with
+                                   | conj _ HP =>
+                                       match HP with
+                                       | conj HP _ => HP
+                                       end
+                                   end
+                               end
+                           end
+                       end) I))))
+  | tvec s0 s1 =>
+      fun HP =>
+      conj
+        (allfvImpl_term p_term q_term H_term s0
+           match HP with
+           | conj HP _ => HP
+           end)
+        (conj
+           (allfvImpl_term p_term q_term H_term s1
+              match HP with
+              | conj _ HP => match HP with
+                             | conj HP _ => HP
+                             end
+              end) I)
+  | tvnil s0 =>
+      fun HP =>
+      conj
+        (allfvImpl_term p_term q_term H_term s0
+           match HP with
+           | conj HP _ => HP
+           end) I
+  | tvcons s0 s1 s2 =>
+      fun HP =>
+      conj
+        (allfvImpl_term p_term q_term H_term s0
+           match HP with
+           | conj HP _ => HP
+           end)
+        (conj
+           (allfvImpl_term p_term q_term H_term s1
+              match HP with
+              | conj _ HP => match HP with
+                             | conj HP _ => HP
+                             end
+              end)
+           (conj
+              (allfvImpl_term p_term q_term H_term s2
+                 match HP with
+                 | conj _ HP =>
+                     match HP with
+                     | conj _ HP => match HP with
+                                    | conj HP _ => HP
+                                    end
+                     end
+                 end) I))
+  | tvec_elim s0 s1 s2 s3 s4 =>
       fun HP =>
       conj I
         (conj
@@ -2413,6 +2712,98 @@ allfv_term (funcomp p_term xi_term) s :=
                                end
                            end
                        end) I))))
+  | tvec s0 s1 =>
+      fun H =>
+      conj
+        (allfvRenL_term p_term xi_term s0 match H with
+                                          | conj H _ => H
+                                          end)
+        (conj
+           (allfvRenL_term p_term xi_term s1
+              match H with
+              | conj _ H => match H with
+                            | conj H _ => H
+                            end
+              end) I)
+  | tvnil s0 =>
+      fun H =>
+      conj
+        (allfvRenL_term p_term xi_term s0 match H with
+                                          | conj H _ => H
+                                          end) I
+  | tvcons s0 s1 s2 =>
+      fun H =>
+      conj
+        (allfvRenL_term p_term xi_term s0 match H with
+                                          | conj H _ => H
+                                          end)
+        (conj
+           (allfvRenL_term p_term xi_term s1
+              match H with
+              | conj _ H => match H with
+                            | conj H _ => H
+                            end
+              end)
+           (conj
+              (allfvRenL_term p_term xi_term s2
+                 match H with
+                 | conj _ H =>
+                     match H with
+                     | conj _ H => match H with
+                                   | conj H _ => H
+                                   end
+                     end
+                 end) I))
+  | tvec_elim s0 s1 s2 s3 s4 =>
+      fun H =>
+      conj I
+        (conj
+           (allfvRenL_term p_term xi_term s1
+              match H with
+              | conj _ H => match H with
+                            | conj H _ => H
+                            end
+              end)
+           (conj
+              (allfvRenL_term p_term xi_term s2
+                 match H with
+                 | conj _ H =>
+                     match H with
+                     | conj _ H => match H with
+                                   | conj H _ => H
+                                   end
+                     end
+                 end)
+              (conj
+                 (allfvRenL_term p_term xi_term s3
+                    match H with
+                    | conj _ H =>
+                        match H with
+                        | conj _ H =>
+                            match H with
+                            | conj _ H => match H with
+                                          | conj H _ => H
+                                          end
+                            end
+                        end
+                    end)
+                 (conj
+                    (allfvRenL_term p_term xi_term s4
+                       match H with
+                       | conj _ H =>
+                           match H with
+                           | conj _ H =>
+                               match H with
+                               | conj _ H =>
+                                   match H with
+                                   | conj _ H =>
+                                       match H with
+                                       | conj H _ => H
+                                       end
+                                   end
+                               end
+                           end
+                       end) I))))
   | bot => fun H => I
   | bot_elim s0 s1 s2 =>
       fun H =>
@@ -2817,6 +3208,98 @@ allfv_term p_term (ren_term xi_term s) :=
                                           | conj H _ => H
                                           end) I
   | tnat_elim s0 s1 s2 s3 s4 =>
+      fun H =>
+      conj I
+        (conj
+           (allfvRenR_term p_term xi_term s1
+              match H with
+              | conj _ H => match H with
+                            | conj H _ => H
+                            end
+              end)
+           (conj
+              (allfvRenR_term p_term xi_term s2
+                 match H with
+                 | conj _ H =>
+                     match H with
+                     | conj _ H => match H with
+                                   | conj H _ => H
+                                   end
+                     end
+                 end)
+              (conj
+                 (allfvRenR_term p_term xi_term s3
+                    match H with
+                    | conj _ H =>
+                        match H with
+                        | conj _ H =>
+                            match H with
+                            | conj _ H => match H with
+                                          | conj H _ => H
+                                          end
+                            end
+                        end
+                    end)
+                 (conj
+                    (allfvRenR_term p_term xi_term s4
+                       match H with
+                       | conj _ H =>
+                           match H with
+                           | conj _ H =>
+                               match H with
+                               | conj _ H =>
+                                   match H with
+                                   | conj _ H =>
+                                       match H with
+                                       | conj H _ => H
+                                       end
+                                   end
+                               end
+                           end
+                       end) I))))
+  | tvec s0 s1 =>
+      fun H =>
+      conj
+        (allfvRenR_term p_term xi_term s0 match H with
+                                          | conj H _ => H
+                                          end)
+        (conj
+           (allfvRenR_term p_term xi_term s1
+              match H with
+              | conj _ H => match H with
+                            | conj H _ => H
+                            end
+              end) I)
+  | tvnil s0 =>
+      fun H =>
+      conj
+        (allfvRenR_term p_term xi_term s0 match H with
+                                          | conj H _ => H
+                                          end) I
+  | tvcons s0 s1 s2 =>
+      fun H =>
+      conj
+        (allfvRenR_term p_term xi_term s0 match H with
+                                          | conj H _ => H
+                                          end)
+        (conj
+           (allfvRenR_term p_term xi_term s1
+              match H with
+              | conj _ H => match H with
+                            | conj H _ => H
+                            end
+              end)
+           (conj
+              (allfvRenR_term p_term xi_term s2
+                 match H with
+                 | conj _ H =>
+                     match H with
+                     | conj _ H => match H with
+                                   | conj H _ => H
+                                   end
+                     end
+                 end) I))
+  | tvec_elim s0 s1 s2 s3 s4 =>
       fun H =>
       conj I
         (conj
