theories/TermMode.v
@@ -46,6 +46,10 @@ Section Mode.
     | tzero => mType
     | tsucc n => mType
     | tnat_elim m n P z s => m
+    | tvec A n => mKind
+    | tvnil A => mType
+    | tvcons a n v => mType
+    | tvec_elim m v P z s => m
     | bot => mKind
     | bot_elim m A p => m
     end.
